
 2024-11-21 11:59

Tags:

## Examples
- $f\left(x\right)=3\sqrt{x}$
		$g\left(x\right)=-10\sqrt{x}$
			$\left(f+g\right)\left(x\right)=3\sqrt{x}+\left(-10\sqrt{x}\right)$
					$\left(f+g\right)\left(x\right)=-7\sqrt{x}$
					$\left(f+g\right)\left(4\right)=-7\sqrt4$
						$=-7\left(2\right)$
						$=-14$

- $f\left(x\right)=x^2$ $g\left(x\right)=\sqrt{x}$
	$fg\left(x\right)=x^2\cdot\sqrt{x}$

- $f\left(x\right)=6x$ $g\left(x\right)=x^{\left(\frac34\right)}$
	$\left(\frac{f}{g}\right)\left(x\right)=\frac{6x}{x}$
		l
# References:

